Also establish Closed and to_val _ = Some _ via reification.

heap_lang/tactics.v
@@ -1,6 +1,197 @@
-From iris.heap_lang Require Export substitution.
+From iris.heap_lang Require Export lang.
 From iris.prelude Require Import fin_maps.
 Import heap_lang.
+
+Module W.
+Inductive expr :=
+  | Val (v : val)
+  | ClosedExpr (e : heap_lang.expr) `{!Closed [] e}
+  (* Base lambda calculus *)
+  | Var (x : string)
+  | Rec (f x : binder) (e : expr)
+  | App (e1 e2 : expr)
+  (* Base types and their operations *)
+  | Lit (l : base_lit)
+  | UnOp (op : un_op) (e : expr)
+  | BinOp (op : bin_op) (e1 e2 : expr)
+  | If (e0 e1 e2 : expr)
+  (* Products *)
+  | Pair (e1 e2 : expr)
+  | Fst (e : expr)
+  | Snd (e : expr)
+  (* Sums *)
+  | InjL (e : expr)
+  | InjR (e : expr)
+  | Case (e0 : expr) (e1 : expr) (e2 : expr)
+  (* Concurrency *)
+  | Fork (e : expr)
+  (* Heap *)
+  | Alloc (e : expr)
+  | Load (e : expr)
+  | Store (e1 : expr) (e2 : expr)
+  | CAS (e0 : expr) (e1 : expr) (e2 : expr).
+
+Fixpoint to_expr (e : expr) : heap_lang.expr :=
+  match e with
+  | Val v => of_val v
+  | ClosedExpr e _ => e
+  | Var x => heap_lang.Var x
+  | Rec f x e => heap_lang.Rec f x (to_expr e)
+  | App e1 e2 => heap_lang.App (to_expr e1) (to_expr e2)
+  | Lit l => heap_lang.Lit l
+  | UnOp op e => heap_lang.UnOp op (to_expr e)
+  | BinOp op e1 e2 => heap_lang.BinOp op (to_expr e1) (to_expr e2)
+  | If e0 e1 e2 => heap_lang.If (to_expr e0) (to_expr e1) (to_expr e2)
+  | Pair e1 e2 => heap_lang.Pair (to_expr e1) (to_expr e2)
+  | Fst e => heap_lang.Fst (to_expr e)
+  | Snd e => heap_lang.Snd (to_expr e)
+  | InjL e => heap_lang.InjL (to_expr e)
+  | InjR e => heap_lang.InjR (to_expr e)
+  | Case e0 e1 e2 => heap_lang.Case (to_expr e0) (to_expr e1) (to_expr e2)
+  | Fork e => heap_lang.Fork (to_expr e)
+  | Alloc e => heap_lang.Alloc (to_expr e)
+  | Load e => heap_lang.Load (to_expr e)
+  | Store e1 e2 => heap_lang.Store (to_expr e1) (to_expr e2)
+  | CAS e0 e1 e2 => heap_lang.CAS (to_expr e0) (to_expr e1) (to_expr e2)
+  end.
+
+Ltac of_expr e :=
+  lazymatch e with
+  | heap_lang.Var ?x => constr:(Var x)
+  | heap_lang.Rec ?f ?x ?e => let e := of_expr e in constr:(Rec f x e)
+  | heap_lang.App ?e1 ?e2 =>
+     let e1 := of_expr e1 in let e2 := of_expr e2 in constr:(App e1 e2)
+  | heap_lang.Lit ?l => constr:(Lit l)
+  | heap_lang.UnOp ?op ?e => let e := of_expr e in constr:(UnOp op e)
+  | heap_lang.BinOp ?op ?e1 ?e2 =>
+     let e1 := of_expr e1 in let e2 := of_expr e2 in constr:(BinOp op e1 e2)
+  | heap_lang.If ?e0 ?e1 ?e2 =>
+     let e0 := of_expr e0 in let e1 := of_expr e1 in let e2 := of_expr e2 in
+     constr:(If e0 e1 e2)
+  | heap_lang.Pair ?e1 ?e2 =>
+     let e1 := of_expr e1 in let e2 := of_expr e2 in constr:(Pair e1 e2)
+  | heap_lang.Fst ?e => let e := of_expr e in constr:(Fst e)
+  | heap_lang.Snd ?e => let e := of_expr e in constr:(Snd e)
+  | heap_lang.InjL ?e => let e := of_expr e in constr:(InjL e)
+  | heap_lang.InjR ?e => let e := of_expr e in constr:(InjR e)
+  | heap_lang.Case ?e0 ?e1 ?e2 =>
+     let e0 := of_expr e0 in let e1 := of_expr e1 in let e2 := of_expr e2 in
+     constr:(Case e0 e1 e2)
+  | heap_lang.Fork ?e => let e := of_expr e in constr:(Fork e)
+  | heap_lang.Alloc ?e => let e := of_expr e in constr:(Alloc e)
+  | heap_lang.Load ?e => let e := of_expr e in constr:(Load e)
+  | heap_lang.Store ?e1 ?e2 =>
+     let e1 := of_expr e1 in let e2 := of_expr e2 in constr:(Store e1 e2)
+  | heap_lang.CAS ?e0 ?e1 ?e2 =>
+     let e0 := of_expr e0 in let e1 := of_expr e1 in let e2 := of_expr e2 in
+     constr:(CAS e0 e1 e2)
+  | to_expr ?e => e
+  | of_val ?v => constr:(Val v)
+  | _ => constr:(ltac:(
+     match goal with H : Closed [] e |- _ => exact (@ClosedExpr e H) end))
+  end.
+
+Fixpoint is_closed (X : list string) (e : expr) : bool :=
+  match e with
+  | Val _ | ClosedExpr _ _ => true
+  | Var x => bool_decide (x ∈ X)
+  | Rec f x e => is_closed (f :b: x :b: X) e
+  | Lit _ => true
+  | UnOp _ e | Fst e | Snd e | InjL e | InjR e | Fork e | Alloc e | Load e =>
+     is_closed X e
+  | App e1 e2 | BinOp _ e1 e2 | Pair e1 e2 | Store e1 e2 =>
+     is_closed X e1 && is_closed X e2
+  | If e0 e1 e2 | Case e0 e1 e2 | CAS e0 e1 e2 =>
+     is_closed X e0 && is_closed X e1 && is_closed X e2
+  end.
+Lemma is_closed_correct X e : is_closed X e → heap_lang.is_closed X (to_expr e).
+Proof.
+  revert X.
+  induction e; naive_solver eauto using is_closed_of_val, is_closed_weaken_nil.
+Qed.
+
+Fixpoint to_val (e : expr) : option val :=
+  match e with
+  | Val v => Some v
+  | Rec f x e =>
+     if decide (is_closed (f :b: x :b: []) e) is left H
+     then Some (@RecV f x (to_expr e) (is_closed_correct _ _ H)) else None
+  | Lit l => Some (LitV l)
+  | Pair e1 e2 => v1 ← to_val e1; v2 ← to_val e2; Some (PairV v1 v2)
+  | InjL e => InjLV <$> to_val e
+  | InjR e => InjRV <$> to_val e
+  | _ => None
+  end.
+Lemma to_val_Some e v :
+  to_val e = Some v → heap_lang.to_val (to_expr e) = Some v.
+Proof.
+  revert v. induction e; intros; simplify_option_eq; rewrite ?to_of_val; auto.
+  - do 2 f_equal. apply proof_irrel.
+  - exfalso. unfold Closed in *; eauto using is_closed_correct.
+Qed.
+
+Fixpoint subst (x : string) (es : expr) (e : expr)  : expr :=
+  match e with
+  | Val v => Val v
+  | ClosedExpr e H => @ClosedExpr e H
+  | Var y => if decide (x = y) then es else Var y
+  | Rec f y e =>
+     Rec f y $ if decide (BNamed x ≠ f ∧ BNamed x ≠ y) then subst x es e else e
+  | App e1 e2 => App (subst x es e1) (subst x es e2)
+  | Lit l => Lit l
+  | UnOp op e => UnOp op (subst x es e)
+  | BinOp op e1 e2 => BinOp op (subst x es e1) (subst x es e2)
+  | If e0 e1 e2 => If (subst x es e0) (subst x es e1) (subst x es e2)
+  | Pair e1 e2 => Pair (subst x es e1) (subst x es e2)
+  | Fst e => Fst (subst x es e)
+  | Snd e => Snd (subst x es e)
+  | InjL e => InjL (subst x es e)
+  | InjR e => InjR (subst x es e)
+  | Case e0 e1 e2 => Case (subst x es e0) (subst x es e1) (subst x es e2)
+  | Fork e => Fork (subst x es e)
+  | Alloc e => Alloc (subst x es e)
+  | Load e => Load (subst x es e)
+  | Store e1 e2 => Store (subst x es e1) (subst x es e2)
+  | CAS e0 e1 e2 => CAS (subst x es e0) (subst x es e1) (subst x es e2)
+  end.
+Lemma to_expr_subst x er e :
+  to_expr (subst x er e) = heap_lang.subst x (to_expr er) (to_expr e).
+Proof.
+  induction e; simpl; repeat case_decide;
+    f_equal; auto using is_closed_nil_subst, is_closed_of_val, eq_sym.
+Qed.
+End W.
+
+Ltac solve_closed :=
+  match goal with
+  | |- Closed ?X ?e =>
+     let e' := W.of_expr e in change (Closed X (W.to_expr e'));
+     apply W.is_closed_correct; vm_compute; exact I
+  end.
+Hint Extern 0 (Closed _ _) => solve_closed : typeclass_instances.
+
+Ltac solve_to_val :=
+  try match goal with
+  | |- language.to_val ?e = Some ?v => change (to_val e = Some v)
+  end;
+  match goal with
+  | |- to_val ?e = Some ?v =>
+     let e' := W.of_expr e in change (to_val (W.to_expr e') = Some v);
+     apply W.to_val_Some; simpl; reflexivity
+  end.
+
+(** Substitution *)
+Ltac simpl_subst :=
+  csimpl;
+  repeat match goal with
+  | |- context [subst ?x ?er ?e] =>
+      let er' := W.of_expr er in let e' := W.of_expr e in
+      change (subst x er e) with (subst x (W.to_expr er') (W.to_expr e'));
+      rewrite <-(W.to_expr_subst x); simpl (* ssr rewrite is slower *)
+  end;
+  unfold W.to_expr.
+Arguments W.to_expr : simpl never.
+Arguments subst : simpl never.
 
 (** The tactic [inv_head_step] performs inversion on hypotheses of the
 shape [head_step]. The tactic will discharge head-reductions starting
