heap_lang/lib/par.v
@@ -39,7 +39,7 @@ Lemma wp_par (Ψ1 Ψ2 : val → iProp)
    ∀ v1 v2, Ψ1 v1 ★ Ψ2 v2 -★ ▷ Φ (v1,v2)%V)
   ⊢ WP e1 || e2 {{ Φ }}.
 Proof.
-  iIntros (?) "(#Hh&H1&H2&H)". iApply (par_spec Ψ1 Ψ2); [done|apply into_value|].
+  iIntros (?) "(#Hh&H1&H2&H)". iApply (par_spec Ψ1 Ψ2); try wp_done.
   iFrame "Hh H". iSplitL "H1"; by wp_let.
 Qed.
 End proof.
